Corrected preservation type
Signed-off-by: Gavin Zhao <gavinz@brown.edu>

Ltlc/Basic.lean
@@ -48,7 +48,7 @@ inductive HasType : Context → LtlcTerm → LtlcType → Prop
   | lam 
     {Γ x α β body}
     (x_fresh : x ∉ Γ)
-    (v_hastype : HasType (Γ ++ .cons x α .nil) body β)
+    (v_hastype : HasType (.cons x α Γ) body β)
     : HasType Γ (LtlcTerm.lam x α body) (.arrow α β)
   | app 
     {Γ₁ Γ₂ t u α β}
@@ -78,10 +78,11 @@ lemma cons_is_append_single {Γ : Context} {x : String} {α : LtlcType}
 
 lemma nil_append_is_same {Γ : Context} : AssocList.nil ++ Γ = Γ := sorry
 
-theorem subst_preserves_type {Γ₁ Γ₂ x α β e a} 
-  (p1 : HasType (.cons x α Γ₁) e β)
-  (p2 : HasType Γ₂ a α)
-  : HasType (Γ₁ ++ Γ₂) ([x // a] e) β :=
+theorem subst_preserves_type {Γ x α β e a} 
+  /- (x_not_in_Γ₂ : x ∉ Γ₂) -/
+  (p1 : HasType (.cons x α Γ) e β)
+  (p2 : HasType .nil a α)
+  : HasType Γ ([x // a] e) β :=
     match e with 
     | .var y => 
         by 
@@ -90,7 +91,6 @@ theorem subst_preserves_type {Γ₁ Γ₂ x α β e a}
             rw [heq] at p1 
             cases p1 with 
             | var => 
-                rw [nil_append_is_same]
                 exact p2
           . simp [heq]
             cases p1 with
@@ -98,20 +98,28 @@ theorem subst_preserves_type {Γ₁ Γ₂ x α β e a}
     | .lam z γ d =>
         by 
           match p1 with 
-          | @HasType.lam _ _ _ β _ x_fresh d_hastype => 
+          | @HasType.lam _ _ _ μ _ z_fresh d_hastype => 
               simp
               by_cases heq : z = x
               -- `[x // a]λx.y` means the original expression is `λx.λx.y`,
               -- which is clearly ill-typed because the outer `x` can never be
               -- used in `y`!
-              · rw [heq] at x_fresh
-                have x_not_fresh : x ∈ AssocList.cons x α Γ₁ :=
-                  by 
-                    simp [Membership.mem, AssocList.contains]
-                contradiction
-              · simp [heq] 
+              · simp [heq]
+                rw [heq] at d_hastype
                 sorry
-    | .app f u => sorry
+              · simp [heq] 
+                apply HasType.lam 
+                · sorry
+                · show HasType (AssocList.cons z γ Γ) ([x // a] d) μ
+                  observe d2 : HasType (AssocList.cons z γ (AssocList.cons x α Γ)) d μ
+                  have d2_swapped : HasType (AssocList.cons x α (AssocList.cons z γ Γ)) d μ := sorry
+                  exact subst_preserves_type d2_swapped p2
+    | .app f u => 
+        by
+          match p1 with 
+          | @HasType.app _ Γ₁ Γ₂ m n μ ν m_is_fn n_is_ν is_append => 
+              simp
+              _
 
 -- theorem preservation {Γ τ e₁ e₂}
 --   (e₁_is_τ : HasType Γ e₁ τ)
@@ -120,16 +128,99 @@ theorem subst_preserves_type {Γ₁ Γ₂ x α β e a}
 --     match e₁_steps_e₂ with 
 --     | Step.app_left f₁_steps_f₂ => 
 --         match e₁_is_τ with 
---         | HasType.app f₁_is_fn e_is_ty => 
---             HasType.app (preservation f₁_is_fn f₁_steps_f₂) e_is_ty
+--         | HasType.app f₁_is_fn e_is_ty is_append => 
+--             HasType.app (preservation f₁_is_fn f₁_steps_f₂) e_is_ty is_append
 --     | Step.app_right u₁_steps_u₂ =>
 --         match e₁_is_τ with 
---         | HasType.app f_is_fn u₁_is_ty => 
---             HasType.app f_is_fn (preservation u₁_is_ty u₁_steps_u₂)
+--         | HasType.app f_is_fn u₁_is_ty is_append => 
+--             HasType.app f_is_fn (preservation u₁_is_ty u₁_steps_u₂) is_append
 --     | @Step.app_lam x α e a => 
 --         match e₁_is_τ with 
---         | @HasType.app Γ₁ Γ₂ _ _ _ β f_is_fn a_is_α => 
+--         | @HasType.app Γ Γ₁ Γ₂ _ _ _ β f_is_fn a_is_α is_append => 
 --             match f_is_fn with 
---             | @HasType.lam _ _ _ _ _ x_fresh bty => 
---                 subst_preserves_type bty a_is_α
-    
+--             | @HasType.lam _ _ _ _ _ bty _ => 
+--                 by
+--                   have is_same : context_append Γ₁ AssocList.nil ++ Γ₂ = Γ :=
+--                     by
+--                       simp [context_append]
+--                       exact Eq.symm is_append
+--                   rw [←is_same]
+--                   _
+
+-- lemma subst_lemma {x e a α β} 
+--   (e_is_β_with_α : HasType (.cons x α .nil) e β )
+--   (v_is_α : HasType .nil a α)
+--   : HasType .nil ([x // a]e) β := 
+--     match e with 
+--     | .var y => 
+--         by 
+--           by_cases heq : y = x 
+--           . simp [heq]
+--             rw [heq] at e_is_β_with_α
+--             cases e_is_β_with_α with 
+--             | var => exact v_is_α
+--           . simp [heq]
+--             cases e_is_β_with_α with
+--             | var => contradiction
+--     | .lam z γ d => 
+--         by
+--           match e_is_β_with_α with 
+--           | @HasType.lam _ _ _ μ _ z_fresh d_is_μ =>
+--               simp 
+--               by_cases heq : z = x 
+--               -- `[x // a]λx.y` means the original expression is `λx.λx.y`,
+--               -- which is clearly ill-typed because the outer `x` can never be
+--               -- used in `y`!
+--               · simp [heq]
+--                 rw [heq] at d_is_μ 
+--                 have z_not_fresh : z ∈ AssocList.cons x α AssocList.nil :=
+--                   by 
+--                     rw [heq]
+--                     simp [Membership.mem, AssocList.contains]
+--                 contradiction
+--               · simp [heq]
+--                 apply HasType.lam 
+--                 · simp [Membership.mem, AssocList.contains]
+--                 · rw [nil_append_is_same]
+--                   _
+--     | _ => sorry
+
+theorem preservation {τ e₁ e₂}
+  (e₁_is_τ : HasType .nil e₁ τ)
+  (e₁_steps_e₂ : Step e₁ e₂)
+  : HasType .nil e₂ τ := 
+    match e₁_steps_e₂ with 
+    | @Step.app_left f₁ f₂ e f₁_steps_f₂ => 
+        match e₁_is_τ with 
+        | @HasType.app _ Γ₁ Γ₂ _ _ α β f₁_is_fn e_is_ty nil_is_Γ₁_append_Γ₂ => 
+            by
+              have Γ₁_is_nil : Γ₁ = AssocList.nil := sorry
+              have Γ₂_is_nil : Γ₂ = AssocList.nil := sorry
+              rw [Γ₁_is_nil] at f₁_is_fn
+              rw [Γ₁_is_nil] at nil_is_Γ₁_append_Γ₂
+              exact HasType.app (preservation f₁_is_fn f₁_steps_f₂) e_is_ty nil_is_Γ₁_append_Γ₂
+    | @Step.app_right f u₁ u₂ u₁_steps_u₂ =>
+        match e₁_is_τ with 
+        | @HasType.app _ Γ₁ Γ₂ _ _ α β f_is_fn u₁_is_α nil_is_Γ₁_append_Γ₂ => 
+            by
+              have Γ₂_is_nil : Γ₂ = AssocList.nil := sorry
+              rw [Γ₂_is_nil] at u₁_is_α
+              rw [Γ₂_is_nil] at nil_is_Γ₁_append_Γ₂
+              exact HasType.app f_is_fn (preservation u₁_is_α u₁_steps_u₂) nil_is_Γ₁_append_Γ₂
+    | @Step.app_lam x α e a => 
+        match e₁_is_τ with 
+        | @HasType.app _ Γ₁ Γ₂ _ _ _ β f_is_fn a_is_α Γ_is_Γ₁_append_Γ₂ => 
+            match f_is_fn with 
+            | @HasType.lam _ _ _ _ _ _ bty => 
+                by
+                  -- have is_same : context_append Γ₁ AssocList.nil ++ Γ₂ = Γ :=
+                  --   by
+                  --     simp [context_append]
+                  --     exact Eq.symm Γ_is_Γ₁_append_Γ₂
+                  -- rw [←is_same]
+                  have Γ₁_is_nil : Γ₁ = AssocList.nil := sorry
+                  have Γ₂_is_nil : Γ₂ = AssocList.nil := sorry
+                  rw [←Γ₁_is_nil]
+                  apply subst_preserves_type bty
+                  rw [←Γ₂_is_nil]
+                  exact a_is_α
